Clean up grammar implementations
Split out the tests, consolidate imports, etc.

src/Parsers/Grammars/ABStar.v
@@ -1,55 +1,13 @@
 (** * Definition of grammar for regular expression [(ab)*] *)
-Require Import Coq.Strings.String Coq.Strings.Ascii Coq.Lists.List.
-Require Import Fiat.Parsers.ContextFreeGrammar Fiat.Parsers.ContextFreeGrammarNotations.
+Require Import Fiat.Parsers.ContextFreeGrammarNotations.
 
-Set Implicit Arguments.
+Definition ab_star_grammar : grammar ascii :=
+  [[[ ("(ab)*" ::== << nil
+                     | $< "a"%char $ "b"%char $ "(ab)*" >$ >> ) ]]]%grammar.
 
-Section ab_star.
-  Local Open Scope string_scope.
+Local Open Scope list_scope.
 
-  Definition ab_star_grammar : grammar Ascii.ascii :=
-    [[[ ("(ab)*" ::== << nil
-                       | $< "a"%char $ "b"%char $ "(ab)*" >$ >> ) ]]]%grammar.
-
-  Definition ab_star_grammar' : grammar Ascii.ascii :=
-    {| Start_symbol := "(ab)*";
-       Lookup := fun _ => nil::(Terminal "a"%char::Terminal "b"%char::NonTerminal "(ab)*"%string::nil)::nil;
-       Valid_nonterminals := ("(ab)*"::nil)%string |}.
-End ab_star.
-
-Create HintDb cfg discriminated.
-Hint Constructors parse_of parse_of_production parse_of_item : cfg.
-
-Section tests.
-  Example ab_star_parses_empty : parse_of_grammar ""%string ab_star_grammar.
-  Proof.
-    hnf; simpl.
-    repeat constructor.
-  Defined.
-
-  Example ab_star_parses_ab : parse_of_grammar "ab"%string ab_star_grammar.
-  Proof.
-    hnf; simpl.
-    apply ParseTail, ParseHead.
-    apply ParseProductionCons with (n := 1); simpl.
-    { refine (ParseTerminal _ _ _ _); reflexivity. }
-    { apply ParseProductionCons with (n := 1); simpl.
-      { refine (ParseTerminal _ _ _ _); reflexivity. }
-      { apply ParseProductionCons with (n := 1); simpl;
-        repeat (simpl; constructor). } }
-  Defined.
-
-  Example ab_star_parses_abab : parse_of_grammar "abab"%string ab_star_grammar.
-  Proof.
-    hnf; simpl.
-    apply ParseTail, ParseHead.
-    apply ParseProductionCons with (n := 1); simpl.
-    { refine (ParseTerminal _ _ _ _); reflexivity. }
-    { apply ParseProductionCons with (n := 1); simpl.
-      { refine (ParseTerminal _ _ _ _); reflexivity. }
-      { apply ParseProductionCons with (n := 2); simpl;
-        try solve [ repeat (simpl; constructor) ].
-        constructor.
-        apply ab_star_parses_ab. } }
-  Defined.
-End tests.
+Definition ab_star_grammar' : grammar ascii :=
+  {| Start_symbol := "(ab)*";
+     Lookup := fun _ => nil::(Terminal "a"%char::Terminal "b"%char::NonTerminal "(ab)*"%string::nil)::nil;
+     Valid_nonterminals := ("(ab)*"::nil)%string |}.
