src/Parsers/Grammars/ExpressionNumPlus.v
@@ -1,50 +1,9 @@
 (** * Definition of grammar for expressions involving plus *)
-Require Import Coq.Strings.String Coq.Strings.Ascii Coq.Lists.List.
-Require Import Fiat.Parsers.ContextFreeGrammar Fiat.Parsers.ContextFreeGrammarNotations.
+Require Import Fiat.Parsers.ContextFreeGrammarNotations.
 
-Set Implicit Arguments.
-
-Section num_plus.
-  Local Open Scope string_scope.
-  Local Open Scope grammar_scope.
-
-  Definition plus_expr_grammar : grammar Ascii.ascii :=
-    [[[ ("expr" ::== << $< "number" >$
-                      | $< "number" $ #"+" $ "expr" >$ >>);;
-        ("digit" ::== << $< #"0" >$ | $< #"1" >$ | $< #"2" >$ | $< #"3" >$ | $< #"4" >$ | $< #"5" >$ | $< #"6" >$ | $< #"7" >$ | $< #"8" >$ | $< #"9" >$ >>);;
-        ("number" ::== << $< "digit" >$ | $< "digit" $ "number" >$ >>)
-    ]]].
-End num_plus.
-
-Section tests.
-  Local Arguments append : simpl never.
-
-  Local Ltac fin :=
-    repeat first [ idtac;
-                   (lazymatch goal with
-                   | [ |- parse_of_production _ ?s (Terminal _ :: _) ]
-                     => apply ParseProductionCons with (n := 1)
-                   | [ |- parse_of_production _ ?s (_ :: nil) ]
-                     => apply ParseProductionCons with (n := String.length s)
-                   | [ |- parse_of_production _ ?s (_ :: Terminal _ :: nil) ]
-                     => apply ParseProductionCons with (n := String.length s - 1)
-                   | _ => apply ParseProductionCons with (n := 1); solve [ fin ]
-                    end)
-                 | apply ParseProductionNil
-                 | refine (ParseTerminal _ _ _)
-                 | refine (ParseNonTerminal _ _)
-                 | progress simpl
-                 | solve [ constructor (solve [ fin ]) ] ].
-
-  Example plus_expr_parses_1 : parse_of_grammar "1+2+3+4+5"%string plus_expr_grammar.
-  Proof.
-    hnf; simpl.
-    apply ParseTail, ParseHead.
-    match goal with
-      | [ |- parse_of_production _ ?s _ ] => set (n := s)
-    end.
-    change n with ("1" ++ ("+" ++ ("2" ++ ("+" ++ ("3" ++ ("+" ++ ("4" ++ ("+" ++ "5"))))))))%string; subst n.
-    simpl.
-    fin.
-  Defined.
-End tests.
+Definition plus_expr_grammar : grammar ascii :=
+  [[[ ("expr" ::== << $< "number" >$
+                   | $< "number" $ #"+" $ "expr" >$ >>);;
+      ("digit" ::== << $< #"0" >$ | $< #"1" >$ | $< #"2" >$ | $< #"3" >$ | $< #"4" >$ | $< #"5" >$ | $< #"6" >$ | $< #"7" >$ | $< #"8" >$ | $< #"9" >$ >>);;
+      ("number" ::== << $< "digit" >$ | $< "digit" $ "number" >$ >>)
+  ]]].
