src/Parsers/Grammars/ExpressionNumPlusParen.v
@@ -1,67 +1,11 @@
 (** * Definition of grammar for expressions involving parentheses and plus *)
-Require Import Coq.Strings.String Coq.Strings.Ascii Coq.Lists.List.
-Require Import Fiat.Parsers.ContextFreeGrammar Fiat.Parsers.ContextFreeGrammarNotations.
+Require Import Fiat.Parsers.ContextFreeGrammarNotations.
 
-Set Implicit Arguments.
-
-Section num_plus_paren.
-  Local Open Scope string_scope.
-  Local Open Scope grammar_scope.
-
-  Definition plus_expr_grammar : grammar Ascii.ascii :=
-    [[[ ("expr" ::== << $< "pexpr" >$
-                      | $< "pexpr" $ #"+" $ "expr" >$ >>);;
-        ("pexpr" ::== << $< "number" >$
-                       | $< #"(" $ "expr" $ #")" >$ >>);;
-        ("digit" ::== << $< #"0" >$ | $< #"1" >$ | $< #"2" >$ | $< #"3" >$ | $< #"4" >$ | $< #"5" >$ | $< #"6" >$ | $< #"7" >$ | $< #"8" >$ | $< #"9" >$ >>);;
-        ("number" ::== << $< "digit" >$ | $< "digit" $ "number" >$ >>)
-    ]]].
-End num_plus_paren.
-
-Section tests.
-  Local Arguments append : simpl never.
-
-  Local Ltac fin :=
-    repeat first [ idtac;
-                   (lazymatch goal with
-                   | [ |- parse_of_production _ ?s (Terminal _ :: _) ]
-                     => apply ParseProductionCons with (n := 1)
-                   | [ |- parse_of_production _ ?s (_ :: nil) ]
-                     => apply ParseProductionCons with (n := String.length s)
-                   | [ |- parse_of_production _ ?s (_ :: Terminal _ :: nil) ]
-                     => apply ParseProductionCons with (n := String.length s - 1)
-                    end)
-                 | apply ParseProductionNil
-                 | refine (ParseTerminal _ _ _)
-                 | refine (ParseNonTerminal _ _)
-                 | progress simpl
-                 | solve [ constructor (solve [ fin ]) ] ].
-
-  Example plus_expr_parses_1 : parse_of_grammar "1+(2+3)+4+5"%string plus_expr_grammar.
-  Proof.
-    hnf; simpl.
-    apply ParseTail, ParseHead.
-    match goal with
-      | [ |- parse_of_production _ ?s _ ] => set (n := s)
-    end.
-    change n with (((("1"))) ++ ("+" ++ (("(" ++ ((((("2"))) ++ ("+" ++ ("3"))) ++ ")")) ++ ("+" ++ ("4" ++ ("+" ++ "5"))))))%string; subst n.
-    apply ParseProductionCons with (n := 1); [ solve [ fin ] | simpl ].
-    apply ParseProductionCons with (n := 1); [ solve [ fin ] | simpl ].
-    apply ParseProductionCons with (n := 9); [ | solve [ fin ] ].
-    constructor; simpl.
-    apply ParseTail, ParseHead.
-    apply ParseProductionCons with (n := 5); simpl.
-    { constructor; simpl.
-      apply ParseTail, ParseHead.
-      apply ParseProductionCons with (n := 1); [ solve [ fin ] | simpl ].
-      apply ParseProductionCons with (n := 3); simpl; [ | solve [ fin ] ].
-      constructor; simpl.
-      apply ParseTail, ParseHead; fin.
-      apply ParseProductionCons with (n := 1); fin. }
-    { apply ParseProductionCons with (n := 1); simpl; [ solve [ fin ] | ].
-      apply ParseProductionCons with (n := 3); simpl; [ | solve [ fin ] ].
-      constructor; simpl.
-      apply ParseTail, ParseHead; fin.
-      apply ParseProductionCons with (n := 1); fin. }
-  Defined.
-End tests.
+Definition plus_expr_grammar : grammar Ascii.ascii :=
+  [[[ ("expr" ::== << $< "pexpr" >$
+                    | $< "pexpr" $ #"+" $ "expr" >$ >>);;
+      ("pexpr" ::== << $< "number" >$
+                     | $< #"(" $ "expr" $ #")" >$ >>);;
+      ("digit" ::== << $< #"0" >$ | $< #"1" >$ | $< #"2" >$ | $< #"3" >$ | $< #"4" >$ | $< #"5" >$ | $< #"6" >$ | $< #"7" >$ | $< #"8" >$ | $< #"9" >$ >>);;
+      ("number" ::== << $< "digit" >$ | $< "digit" $ "number" >$ >>)
+  ]]].
