src/Parsers/Grammars/Tests.v
@@ -1,0 +1,197 @@
+Require Import Coq.Strings.String Coq.Strings.Ascii Coq.Lists.List.
+Require Import Fiat.Parsers.ContextFreeGrammar Fiat.Parsers.ContextFreeGrammarNotations.
+Require Import Fiat.Common.StringOperations Fiat.Common.StringFacts.
+Require Import Fiat.Parsers.StringLike.Properties.
+Require Import Fiat.Parsers.StringLike.String.
+
+Require Import Fiat.Parsers.Grammars.ABStar.
+Require Import Fiat.Parsers.Grammars.ExpressionNumPlus.
+Require Import Fiat.Parsers.Grammars.ExpressionNumPlusParen.
+Require Import Fiat.Parsers.Grammars.ExpressionParen.
+
+Section ab_star.
+  Example ab_star_parses_empty : parse_of_grammar ""%string ab_star_grammar.
+  Proof.
+    hnf; simpl.
+    repeat constructor.
+  Defined.
+
+  Example ab_star_parses_ab : parse_of_grammar "ab"%string ab_star_grammar.
+  Proof.
+    hnf; simpl.
+    apply ParseTail, ParseHead.
+    apply ParseProductionCons with (n := 1); simpl.
+    { refine (ParseTerminal _ _ _ _); reflexivity. }
+    { apply ParseProductionCons with (n := 1); simpl.
+      { refine (ParseTerminal _ _ _ _); reflexivity. }
+      { apply ParseProductionCons with (n := 1); simpl;
+        repeat (simpl; constructor). } }
+  Defined.
+
+  Example ab_star_parses_abab : parse_of_grammar "abab"%string ab_star_grammar.
+  Proof.
+    hnf; simpl.
+    apply ParseTail, ParseHead.
+    apply ParseProductionCons with (n := 1); simpl.
+    { refine (ParseTerminal _ _ _ _); reflexivity. }
+    { apply ParseProductionCons with (n := 1); simpl.
+      { refine (ParseTerminal _ _ _ _); reflexivity. }
+      { apply ParseProductionCons with (n := 2); simpl;
+        try solve [ repeat (simpl; constructor) ].
+        constructor.
+        apply ab_star_parses_ab. } }
+  Defined.
+End ab_star.
+
+Section num_paren.
+  (*Context {HSL : StringLike Ascii.ascii} {HSLP : StringLikeProperties Ascii.ascii}.*)
+  Local Arguments append : simpl never.
+
+  Local Ltac safe_step :=
+    idtac;
+    (match goal with
+       | _ => reflexivity
+       | [ |- parse_of_production _ ?s (Terminal _ :: _) ]
+         => apply ParseProductionCons with (n := 1)
+       | [ |- parse_of_production _ ?s (_ :: nil) ]
+         => apply ParseProductionCons with (n := String.length s)
+       | [ |- parse_of_production _ ?s (_ :: nil) ]
+         => apply ParseProductionCons with (n := StringLike.length s)
+       | [ |- parse_of_production _ ?s (_ :: Terminal _ :: nil) ]
+         => apply ParseProductionCons with (n := StringLike.length s - 1)
+       | [ |- parse_of_production _ _ nil ]
+         => apply ParseProductionNil
+       | [ |- parse_of_item _ _ (Terminal _) ]
+         => apply ParseTerminal
+       | [ |- parse_of_item _ _ (NonTerminal _) ]
+         => apply ParseNonTerminal
+       | [ |- is_true (is_char (take 1 _) _) ] => apply get_0
+       (*| [ |- context[StringLike.get _ (of_string _)] ] => (rewrite !get_of_string; simpl)*)
+       (*| [ |- context[StringLike.length _] ] => (progress rewrite ?take_length, ?drop_length, ?of_string_length; simpl List.length; simpl minus)*)
+       (*| [ |- context[StringLike.get _ _] ] => (progress repeat rewrite ?take_of_string, ?drop_of_string; simpl; rewrite get_of_string; reflexivity)*)
+       | _ => progress simpl
+     end).
+
+  Local Ltac fin :=
+    repeat first [ safe_step
+                 | apply ParseProductionCons with (n := 1); solve [ fin ]
+                 | constructor (solve [ fin ]) ].
+
+  Example paren_expr_parses_1 : parse_of_grammar ((*of_string*) ((*list_of_string*) "(((123)))"%string)) paren_expr_grammar.
+  Proof.
+    hnf; simpl.
+    apply ParseTail, ParseHead; repeat safe_step; [].
+    apply ParseTail, ParseHead; repeat safe_step; [].
+    apply ParseTail, ParseHead; repeat safe_step; [].
+    apply ParseHead; repeat safe_step; [].
+    apply ParseTail, ParseHead; repeat safe_step; [].
+    apply ParseProductionCons with (n := 1); repeat safe_step; [ fin | ].
+    apply ParseTail, ParseHead; repeat safe_step; [].
+    apply ParseProductionCons with (n := 1); repeat safe_step; [ fin | ].
+    apply ParseHead; repeat safe_step; [].
+    apply ParseTail, ParseTail, ParseTail, ParseHead; repeat safe_step.
+  Qed.
+End num_paren.
+
+Section num_plus.
+  Local Arguments append : simpl never.
+
+  Local Ltac fin'0 tac :=
+    repeat first [ idtac;
+                   (lazymatch goal with
+                   | [ |- parse_of_production _ ?s (Terminal _ :: _) ]
+                     => apply ParseProductionCons with (n := 1)
+                   | [ |- parse_of_production _ ?s (_ :: nil) ]
+                     => apply ParseProductionCons with (n := String.length s)
+                   | [ |- parse_of_production _ ?s (_ :: Terminal _ :: nil) ]
+                     => apply ParseProductionCons with (n := String.length s - 1)
+                   | _ => (apply ParseProductionCons with (n := 1); solve [ tac ])
+                    end)
+                 | idtac;
+                   match goal with
+                     | [ |- _ = _ ] => reflexivity
+                     | [ |- is_true true ] => reflexivity
+                   end
+                 | apply ParseProductionNil
+                 | apply ParseTerminal
+                 | apply ParseNonTerminal
+                 | progress simpl ].
+
+  Local Ltac fin' := idtac; fin'0 fin'.
+
+  Local Ltac fin :=
+    repeat first [ progress fin'0 fin
+                 | solve [ constructor (solve [ fin ]) ] ].
+
+  Example plus_expr_parses_1 : parse_of_grammar "1+2+3+4+5"%string plus_expr_grammar.
+  Proof.
+    hnf; simpl.
+    apply ParseTail, ParseHead.
+    match goal with
+      | [ |- parse_of_production _ ?s _ ] => set (n := s)
+    end.
+    change n with ("1" ++ ("+" ++ ("2" ++ ("+" ++ ("3" ++ ("+" ++ ("4" ++ ("+" ++ "5"))))))))%string; subst n.
+    simpl.
+    fin'.
+    apply ParseProductionCons with (n := 1); fin'.
+    { apply ParseHead; fin. }
+    apply ParseTail, ParseHead; fin'.
+    apply ParseProductionCons with (n := 1); fin'.
+    { apply ParseHead; fin. }
+    apply ParseTail, ParseHead; fin'.
+    apply ParseProductionCons with (n := 1); fin'.
+    { apply ParseHead; fin. }
+    apply ParseTail, ParseHead; fin'.
+    apply ParseProductionCons with (n := 1); fin'.
+    { apply ParseHead; fin. }
+    apply ParseHead; fin.
+  Defined.
+End num_plus.
+
+Section num_plus_paren.
+  Local Arguments append : simpl never.
+
+  Local Ltac fin :=
+    repeat first [ idtac;
+                   (lazymatch goal with
+                   | [ |- parse_of_production _ ?s (Terminal _ :: _) ]
+                     => apply ParseProductionCons with (n := 1)
+                   | [ |- parse_of_production _ ?s (_ :: nil) ]
+                     => apply ParseProductionCons with (n := String.length s)
+                   | [ |- parse_of_production _ ?s (_ :: Terminal _ :: nil) ]
+                     => apply ParseProductionCons with (n := String.length s - 1)
+                    end)
+                 | apply ParseProductionNil
+                 | refine (ParseTerminal _ _ _)
+                 | refine (ParseNonTerminal _ _)
+                 | progress simpl
+                 | solve [ constructor (solve [ fin ]) ] ].
+
+  Example plus_paren_expr_parses_1 : parse_of_grammar "1+(2+3)+4+5"%string plus_expr_grammar.
+  Proof.
+    hnf; simpl.
+    apply ParseTail, ParseHead.
+    match goal with
+      | [ |- parse_of_production _ ?s _ ] => set (n := s)
+    end.
+    change n with (((("1"))) ++ ("+" ++ (("(" ++ ((((("2"))) ++ ("+" ++ ("3"))) ++ ")")) ++ ("+" ++ ("4" ++ ("+" ++ "5"))))))%string; subst n.
+    apply ParseProductionCons with (n := 1); [ solve [ fin ] | simpl ].
+    apply ParseProductionCons with (n := 1); [ solve [ fin ] | simpl ].
+    apply ParseProductionCons with (n := 9); [ | solve [ fin ] ].
+    constructor; simpl.
+    apply ParseTail, ParseHead.
+    apply ParseProductionCons with (n := 5); simpl.
+    { constructor; simpl.
+      apply ParseTail, ParseHead.
+      apply ParseProductionCons with (n := 1); [ solve [ fin ] | simpl ].
+      apply ParseProductionCons with (n := 3); simpl; [ | solve [ fin ] ].
+      constructor; simpl.
+      apply ParseTail, ParseHead; fin.
+      apply ParseProductionCons with (n := 1); fin. }
+    { apply ParseProductionCons with (n := 1); simpl; [ solve [ fin ] | ].
+      apply ParseProductionCons with (n := 3); simpl; [ | solve [ fin ] ].
+      constructor; simpl.
+      apply ParseTail, ParseHead; fin.
+      apply ParseProductionCons with (n := 1); fin. }
+  Defined.
+End num_plus_paren.
